>  A formal power series is a series $A(X)....
>
> Note that Often the an are positives are represent the size of some set we are interested in



For example. Let $a_n$ be the number of lists of $\set{1,2,..,n}$. In this case, $a_n=n!$



We create the power series $A(x) = \sum{}{}$



Note that the only converge out of $x=0$. We don't care. We can (and do) add and multiple formal power series in the obvious way



*Example*

$\sum{a_nx^n} + \sum{b_nx^n} = \sum{(a_n+b_n)x^n}$

$\sum{a_nx^n}\sum{b_nx^n} = (a_0+a_1x + a_2x^2+...) \cdot (b_0 +b_1x +b_2x^2+...)$

$a_{0}b_{0} + (a_{0} b_{1} +a_{1}b_{0})x + (a_0 b_{2} + a_1 b_1 + a_2 b_0)x^2$

$=\sum_{n=0}^{\infin}{a_kb_{n-k} x^n}$



Note that we often call $x$ an indeterminates, not a variable. 

- A variable is a place holder that we occasionally evaluate at. We (almost never) evaluate of x. Hnece we could
- We could manipulate formal power series algebraically disregarding convergence



*Example*

Let $A(x) = \sum_{n=0}^{\infin} x^n = 1 + x + x^2 +...$

- Notice $xA(x) = x + x^2 + x^3 +...$, which gives $A(x) - xA(x) = 1+ 0x +0x^2 + 0x^3 +.... = 1$

Or equivalentialy

- $(1-x)A(x) = 1$
- $A(x) = \frac{1}{1-x}$ (Not a former power series)
- $(1-x) = \frac{1}{A(x)}$



> Thm. Let $n \geq 0 $ be fixed. Let $a_k$ be the number of subsets of $\set{1,2,...,n}$ of size $k$



Show that $\sum_{k=0}^{\infin} a_k x^k= \sum_{k=0}^{n}a_kx^k=\sum_{k=0}^{n} {n \choose k} x^k = (1+x)^n$

- Note that $k > n$ then, $a_k = 0$. Hence the first equality

- Second equality comes from previous work



Let $P(n)$ be the set of all subsets of $\set{1,2,..,n}$. Let $B =$ set of all $(a_1, ... , a_n)$ with $a_i \in \set{0, 1}$

Let $f(\set{c_1,...,c_k}) = (b_1, ..., b_n)$ where $b_i = 1 : i \in {c_1,...,c_k} | b_i =0 : i \in {b_1,...,b_k}$

Let $ n = 10$

- $f(\set{1,2,5,7}) =  (1,1,0,0,1,0,1,0,0,0)$ 



We see that

- $f^-1((b_1,..,b_n)) = \set{i : b_i = 1}$

- $f^-1((0,1,1,0,1)) = \set{2,3,5}$ where $n=5$



We have

$\sum_{k=0}^{n} c_kx^k = \sum_{k=0}^{n} \sum_{\set{c_1,..,c_k}(|k|)} x^k= \sum_{k=0} ^{\infin}\sum_{(a_1,..b_n) :\sum a_i =k}x^{b_1+...+b_n} = \sum_{b_1..b_n=B}x^{b_1+..+b_n}$

$= \sum_{b_i \in \set{0,1}} x^{b_1+...+b_n} = \sum_{b_1 \in \set{0,1}} \sum_{b_2 \in \set{0,1}} \sum_{b_3 \in \set{0,1}}...\sum_{b_n \in \set{0,1}}x^{b_1 +...+b_n}$

$=\sum_{b_1 \in \set{0,1}}x^{b_1} \sum_{b_2 \in \set{0,1}}x^{b_2} ...\sum_{b_n \in \set{0,1}}x^{b_n} = (1+x)(1+x)...=(1+x)^n$



*Example*

Show that ${m+n \choose k} = \sum_{j=0}^k {m \choose j}{n \choose k-j}$



Ntocie that

 $(i + x^{m+n}) = \sum_{k=0}^{m+n} {m+n \choose k}x^k$

Further

$ (1+x)^{m+n} = (1+x)^m(1+x)^n = \sum_{j=0}^m {m \choose j}x^j \sum_{i=0}^n {n \choose i}x^i$

This gives that

$(1+x)^{m+n} = \sum_{j=0}^m \sum_{i=0}^n {m \choose j} {n \choose i}x^{j+i} = \sum_{k=0}^{m+n}\sum_{i+j=k} {m \choose j}{n \choose i}x^{j+i}$

$= \sum_{k=0}^{m+n} \sum_{i+j=k} {m \choose j}{n \choose k-j}x^k = \sum_{k=0}^{m+n} \sum_{j=0}^{k} {m \choose j}{n \choose k-j}x^k$



By looking at the coefficient in front of $x^k$ we get the left hand side = right hand side. 

- Notation $[x^k](\sum a_kx^k) = a_k=$ coefficient in front of $x^k$



















